src/S4/ops.lean
@@ -1,0 +1,358 @@
+import .size
+open nnf list
+
+namespace list
+universes u v w
+
+variables {α : Type u} {β : Type v} {γ : Type w}
+
+theorem mapp {p : β → Prop} (f : α → β) : Π (l : list α) (h : ∀ x∈l, p (f x)) x, x ∈ list.map f l → p x
+| [] h x := by simp
+| (hd::tl) h x := 
+begin
+  intro hmem, cases hmem,
+  {rw hmem, apply h, simp},
+  {apply mapp tl, intros a ha, apply h, simp [ha], exact hmem}
+end
+
+theorem pmapp {p : β → Prop} {q : α → Prop} (f : Π a, q a → β)  : Π (l : list α) 
+(h : ∀ y (hy : q y) (h₁ : y ∈ l), p (f y hy)) 
+(hf : ∀ y ∈ l, q y) x, x ∈ list.pmap f l hf → p x
+| [] h hf x := by simp
+| (hd::tl) h hf x := 
+begin
+  intro hmem, 
+  cases hmem,
+  {rw hmem, apply h, simp},
+  {apply pmapp tl, intros a ha hamem, 
+   apply h, simp [ha], right, exact hamem, exact hmem}
+end
+
+@[simp] def ne_empty_head : Π l : list α, l ≠ [] → α
+| []       h := by contradiction
+| (a :: l) h := a
+
+end list
+
+@[simp] def unbox : list nnf → list nnf
+| [] := []
+| ((box φ) :: l) := φ :: unbox l
+| (e :: l) := unbox l
+
+theorem unbox_iff : Π {Γ φ}, box φ ∈ Γ ↔ φ ∈ unbox Γ
+| [] φ := begin split, repeat {intro h, simpa using h} end
+| (hd::tl) φ := 
+begin
+  split,
+  { intro h, cases h₁ : hd, 
+    case nnf.box : ψ 
+    { dsimp [unbox], cases h, 
+       {left, rw h₁ at h, injection h},
+       {right, exact (@unbox_iff tl φ).1 h} },
+    all_goals 
+    { dsimp [unbox], cases h, 
+       {rw h₁ at h, contradiction},
+       {exact (@unbox_iff tl φ).1 h} } },
+  { intro h, cases h₁ : hd, 
+    case nnf.box : ψ
+    { rw h₁ at h, dsimp [unbox] at h, cases h, 
+       {simp [h]}, {right, exact (@unbox_iff tl φ).2 h} },
+    all_goals 
+    { rw h₁ at h, dsimp [unbox] at h, right, exact (@unbox_iff tl φ).2 h } }
+end
+
+theorem unbox_size_aux : Π {Γ}, node_size (unbox Γ) ≤ node_size Γ
+| [] := by simp
+| (hd::tl) := 
+begin
+  cases h : hd,
+  case nnf.box : ψ
+  { dsimp, apply add_le_add, 
+     { dsimp [sizeof, has_sizeof.sizeof, nnf.sizeof], 
+       rw add_comm, apply nat.le_succ }, 
+     { apply unbox_size_aux } },
+  all_goals 
+  { dsimp, apply le_add_of_nonneg_of_le, 
+    { dsimp [sizeof, has_sizeof.sizeof, nnf.sizeof], rw add_comm, apply nat.zero_le }, 
+    { apply unbox_size_aux } }
+end
+
+@[simp] def rebox : list nnf → list nnf 
+| [] := []
+| (hd::tl) := box hd :: rebox tl
+
+theorem rebox_unbox_of_mem : Π {Γ} (h : ∀ {φ}, φ ∈ unbox Γ → box φ ∈ Γ), rebox (unbox Γ) ⊆ Γ
+| [] h := by simp
+| (hd::tl) h := 
+begin
+  cases hψ : hd,
+  case nnf.box : φ {dsimp, simp [cons_subset_cons], apply subset_cons_of_subset, apply rebox_unbox_of_mem, simp [unbox_iff]},
+  all_goals {dsimp, apply subset_cons_of_subset, apply rebox_unbox_of_mem, simp [unbox_iff]}
+end
+
+theorem unbox_rebox : Π {Γ}, unbox (rebox Γ) = Γ
+| [] := by simp
+| (hd::tl) := by simp [unbox_rebox]
+
+-- Just that I don't want to say ∃ φ s.t. ...
+def box_only_rebox : Π {Γ}, box_only (rebox Γ)
+| [] := {no_var := by simp, 
+         no_neg := by simp, 
+         no_and := by simp, 
+         no_or  := by simp, 
+         no_dia := by simp}
+| (hd::tl) := 
+begin
+  cases h : hd,
+  all_goals {
+  exact { no_var := begin 
+                      intros n h, cases h, contradiction, 
+                      apply (@box_only_rebox tl).no_var, assumption 
+                    end, 
+          no_neg := begin 
+                      intros n h, cases h, contradiction, 
+                      apply (@box_only_rebox tl).no_neg, assumption 
+                    end,
+          no_and := begin 
+                      intros φ ψ h, cases h, contradiction, 
+                      apply (@box_only_rebox tl).no_and, assumption 
+                    end,
+          no_or := begin 
+                     intros φ ψ h, cases h, contradiction, 
+                     apply (@box_only_rebox tl).no_or, assumption 
+                   end, 
+          no_dia := begin 
+                      intros φ h, cases h, contradiction, 
+                      apply (@box_only_rebox tl).no_dia, assumption 
+                    end} }
+end
+
+theorem rebox_iff : Π {φ Γ}, box φ ∈ rebox Γ ↔ φ ∈ Γ
+| φ [] := by simp
+| φ (hd::tl) := 
+begin
+  split, 
+  {intro h, cases h₁ : hd, 
+   all_goals { cases h, 
+               {left, rw ←h₁, injection h}, 
+               {right,  have := (@rebox_iff φ tl).1, exact this h } }},
+  {intro h, cases h₁ : hd, 
+   all_goals { dsimp, cases h, 
+               {left, rw ←h₁, rw h}, 
+               {right, have := (@rebox_iff φ tl).2, exact this h } } }
+end
+
+@[simp] def undia : list nnf → list nnf
+| [] := []
+| ((dia φ) :: l) := φ :: undia l
+| (e :: l) := undia l
+
+theorem undia_iff : Π {Γ φ}, dia φ ∈ Γ ↔ φ ∈ undia Γ
+| [] φ := begin split, repeat {intro h, simpa using h} end
+| (hd::tl) φ := 
+begin
+  split,
+  { intro h, cases h₁ : hd, 
+    case nnf.dia : ψ 
+    { dsimp [undia], cases h, 
+       {left, rw h₁ at h, injection h},
+       {right, exact (@undia_iff tl φ).1 h} },
+    all_goals 
+    { dsimp [undia], cases h, 
+       {rw h₁ at h, contradiction},
+       {exact (@undia_iff tl φ).1 h} } },
+  { intro h, cases h₁ : hd, 
+    case nnf.dia : ψ
+    { rw h₁ at h, dsimp [undia] at h, cases h, 
+       {simp [h]}, {right, exact (@undia_iff tl φ).2 h} },
+    all_goals 
+    { rw h₁ at h, dsimp [undia] at h, right, exact (@undia_iff tl φ).2 h } }
+end
+
+def get_contra : Π Γ : list nnf, 
+                 psum {p : nat // var p ∈ Γ ∧ neg p ∈ Γ} 
+                      (∀ n, var n ∈ Γ → neg n ∉ Γ)
+| []             := psum.inr $ λ _ h, absurd h $ not_mem_nil _
+| (hd :: tl)     := 
+begin
+  cases h : hd,
+  case nnf.var : n 
+  {apply dite (neg n ∈ tl),
+    {intro t, 
+     exact psum.inl ⟨n, ⟨mem_cons_self _ _, mem_cons_of_mem _ t⟩⟩},
+    {intro e, 
+     cases (get_contra tl),
+     {left, constructor, constructor,
+     apply mem_cons_of_mem, exact val.2.1,
+     apply mem_cons_of_mem, exact val.2.2},
+     {right,
+      intros m hm hin, 
+      by_cases eq : m=n,
+      {apply e, cases hin, contradiction, rw ←eq, assumption},
+      {cases hm, apply eq, injection hm, apply val, exact hm, 
+       cases hin, contradiction, assumption} } }
+  },
+  case nnf.neg : n 
+  { apply dite (var n ∈ tl),
+    { intro t, 
+      exact psum.inl ⟨n, ⟨mem_cons_of_mem _ t, mem_cons_self _ _⟩⟩ },
+    { intro e, 
+      cases (get_contra tl),
+      {left, constructor, constructor,
+      apply mem_cons_of_mem, exact val.2.1,
+      apply mem_cons_of_mem, exact val.2.2 },
+      { right,
+        intros m hm hin, 
+        by_cases eq : m=n,
+        { apply e, cases hm, contradiction, rw ←eq, assumption },
+        { cases hin, apply eq, injection hin, apply val, 
+          swap, exact hin, cases hm, contradiction, assumption } 
+      } 
+    }
+  },
+  all_goals
+  { 
+  cases (get_contra tl),
+  { left, constructor, constructor,
+    apply mem_cons_of_mem, exact val.2.1,
+    apply mem_cons_of_mem, exact val.2.2  },
+  { right,
+    intros m hm hin, 
+    {apply val, swap 3, exact m, 
+    cases hm, contradiction, assumption,
+    cases hin, contradiction, assumption} }
+  }
+end
+
+def get_contra_seqt : Π Γ : sseqt,
+                 psum {p : nat // var p ∈ Γ.m ∧ neg p ∈ Γ.m} 
+                      (∀ n, var n ∈ Γ.m → neg n ∉ Γ.m)
+:= λ Γ, get_contra Γ.m
+
+def get_and : Π Γ : list nnf, 
+              psum {p : nnf × nnf // and p.1 p.2 ∈ Γ} 
+                   (∀ φ ψ, nnf.and φ ψ ∉ Γ)
+| []               := psum.inr $ λ _ _, not_mem_nil _
+| (hd :: tl)       := 
+begin
+  cases h : hd,
+  case nnf.and : φ ψ { left, constructor,swap,
+                       constructor, exact φ, exact ψ, simp
+                     },
+  all_goals 
+  { cases (get_and tl),
+    {left,
+    constructor,
+    apply mem_cons_of_mem,
+    exact val.2},
+    {right, intros γ ψ h, 
+     cases h, contradiction,
+    apply val, assumption }
+  }
+end
+
+def get_and_seqt : Π Γ : sseqt, 
+              psum {p : nnf × nnf // and p.1 p.2 ∈ Γ.m} 
+                   (∀ φ ψ, nnf.and φ ψ ∉ Γ.m)
+:= λ Γ, get_and Γ.m
+
+def get_or : Π Γ : list nnf, 
+              psum {p : nnf × nnf // or p.1 p.2 ∈ Γ} 
+                   (∀ φ ψ, nnf.or φ ψ ∉ Γ)
+| []               := psum.inr $ λ _ _, not_mem_nil _
+| (hd :: tl)       :=
+begin
+  cases h : hd,
+  case nnf.or : φ ψ { left, constructor,swap,
+                       constructor, exact φ, exact ψ, simp },
+  all_goals 
+  { cases (get_or tl),
+    {left,
+    constructor,
+    apply mem_cons_of_mem,
+    exact val.2},
+    {right, intros γ ψ h, 
+     cases h, contradiction,
+    apply val, assumption}
+  }
+end
+
+def get_or_seqt : Π Γ : sseqt,
+              psum {p : nnf × nnf // or p.1 p.2 ∈ Γ.m} 
+                   (∀ φ ψ, nnf.or φ ψ ∉ Γ.m)
+:= λ Γ, get_or Γ.m
+
+def get_dia : Π Γ : list nnf, 
+              psum {p : nnf // dia p ∈ Γ} 
+                   (∀ φ, nnf.dia φ ∉ Γ)
+| []               := psum.inr $ λ _, not_mem_nil _
+| (hd :: tl)       := 
+begin
+  cases h : hd,
+  case nnf.dia : φ { left, constructor, swap, exact φ, simp },
+  all_goals 
+  { cases (get_dia tl),
+    {left,
+    constructor,
+    apply mem_cons_of_mem,
+    exact val.2},
+    {right, intros γ h, 
+     cases h, contradiction,
+     apply val, assumption } }
+end
+
+def get_dia_seqt : Π Γ : sseqt,
+              psum {p : nnf // dia p ∈ Γ.m} 
+                   (∀ φ, nnf.dia φ ∉ Γ.m)
+:= λ Γ, get_dia Γ.m
+
+def get_box : Π Γ : list nnf,
+              psum {l : nnf // box l ∈ Γ} 
+                   (∀ φ, nnf.box φ ∉ Γ)
+| [] := psum.inr $ λ _, not_mem_nil _
+| (hd :: tl) := 
+begin
+  cases h : hd,
+  case nnf.box : φ { left, constructor, swap, exact φ, simp },
+  all_goals 
+  { cases (get_box tl),
+    {left,
+    constructor,
+    apply mem_cons_of_mem,
+    exact val.2},
+    {right, intros γ h, 
+     cases h, contradiction,
+     apply val, assumption } }
+end
+
+def get_box_seqt : Π Γ : sseqt,
+              psum {p : nnf // box p ∈ Γ.m} 
+                   (∀ φ, nnf.box φ ∉ Γ.m)
+:= λ Γ, get_box Γ.m
+
+@[simp] def get_var : list nnf → list ℕ
+| [] := []
+| ((var n) :: l) := n :: get_var l
+| (e :: l) := get_var l
+
+theorem get_var_iff : Π {Γ n}, var n ∈ Γ ↔ n ∈ get_var Γ
+| [] φ := begin split, repeat {intro h, simpa using h} end
+| (hd::tl) φ := 
+begin
+  split,
+  { intro h, cases h₁ : hd, 
+    case nnf.var : n
+    { dsimp, cases h, 
+       {left, rw h₁ at h, injection h},
+       {right, exact (@get_var_iff tl φ).1 h} },
+    all_goals 
+    { dsimp, cases h, 
+       {rw h₁ at h, contradiction},
+       {exact (@get_var_iff tl φ).1 h} } },
+  { intro h, cases h₁ : hd, 
+    case nnf.var : n
+    { rw h₁ at h, dsimp at h, cases h, 
+       {simp [h]}, {right, exact (@get_var_iff tl φ).2 h} },
+    all_goals 
+    { rw h₁ at h, dsimp [undia] at h, right, exact (@get_var_iff tl φ).2 h } }
+end
