src/S4/semantics.lean
@@ -1,0 +1,38 @@
+import .ops
+open subtype nnf model list
+
+def unmodal_seqt (Γ : sseqt) : list sseqt :=
+@list.pmap _ _ (λ φ, φ ∉ Γ.h ∧ dia φ ∈ Γ.m)
+(λ d h,
+({goal := Γ.goal,
+s := some {d := d, b := Γ.b},
+a := {d := d, b := Γ.b} :: Γ.a,
+h := d :: Γ.h,
+b := Γ.b,
+m := d :: Γ.b,
+ndh := begin rw list.nodup_cons, split, exact h.1, exact Γ.ndh end,
+ndb := Γ.ndb,
+sph := begin apply list.cons_subperm_of_mem, apply Γ.ndh, exact h.1, apply mem_closure_dia, apply Γ.sbm, exact h.2,  exact Γ.sph end,
+spb := Γ.spb,
+sbm := begin rw list.cons_subset, split, apply mem_closure_dia, apply Γ.sbm, exact h.2, apply list.subset_of_subperm, exact Γ.spb end
+} : sseqt))
+(filter_undia Γ.h Γ.m)
+(begin
+intros φ hmem,
+split, 
+{apply mem_filter_dia_right, exact hmem},
+{apply mem_filter_dia_right_aux, exact hmem}
+end)
+
+def unmodal_seqt_size (Γ : sseqt) : ∀ (i : sseqt),  i ∈ unmodal_seqt Γ → (prod.measure_lex' sseqt_size i Γ) := 
+list.pmapp _ _ 
+begin 
+intros φ h hmem,
+right, left,
+apply length_sub_lt_of_nodup_subperm,
+{apply Γ.sph},
+{apply mem_closure_dia, apply Γ.sbm, exact h.2},
+{exact h.1},
+{exact Γ.ndh}
+end 
+_
