src/S4/size.lean
@@ -1,0 +1,135 @@
+import .S4_defs 
+open nnf prod list
+
+namespace prod
+
+universe u
+
+def measure_lex {α : Sort u} : (α → ℕ × ℕ) → α → α → Prop :=
+inv_image $ lex (<) (<)
+
+def measure_lex' {α : Sort u} : (α → ℕ × ℕ × ℕ) → α → α → Prop :=
+inv_image $ lex (<) (measure_lex (λ x, x))
+
+def measure_lex_wf {α : Sort u} (f : α → ℕ × ℕ) : well_founded (measure_lex f) :=
+inv_image.wf f (lex_wf nat.lt_wf nat.lt_wf)
+
+def measure_lex_wf' {α : Sort u} (f : α → ℕ × ℕ × ℕ) : well_founded (measure_lex' f) :=
+inv_image.wf f (lex_wf nat.lt_wf (measure_lex_wf (λ x, x)))
+
+end prod
+
+instance : has_well_founded sseqt := 
+⟨prod.measure_lex' sseqt_size, prod.measure_lex_wf' sseqt_size⟩
+-- ⟨ prod.measure_lex seqt_size, prod.measure_lex_wf seqt_size ⟩
+
+lemma size_erase_add_eq_size_sum {φ} : Π (Γ : list nnf) (h : φ ∈ Γ), node_size (Γ.erase φ) + sizeof φ = node_size Γ
+| [] h := absurd h $ not_mem_nil _
+| (hd :: tl) h := 
+begin
+  by_cases eq : φ = hd,
+  {dsimp [list.erase], rw if_pos, rw eq, apply add_comm, rw eq},
+  {dsimp [list.erase], rw if_neg, dsimp, rw [add_assoc],   have : node_size (list.erase tl φ) + sizeof φ = node_size tl,
+    {apply size_erase_add_eq_size_sum, cases h, contradiction, assumption},
+    rw this, intro h', rw h' at eq, contradiction}
+end
+
+theorem split_lt_and_size {φ ψ} (Γ : list nnf) (h : nnf.and φ ψ ∈ Γ) :
+node_size (φ :: ψ :: Γ.erase (nnf.and φ ψ)) < node_size Γ := 
+begin
+  dsimp [node_size],
+  rw ←size_erase_add_eq_size_sum Γ,
+  swap, exact h,
+  rw [←add_assoc, add_comm],
+  apply add_lt_add_left, dsimp [sizeof, has_sizeof.sizeof, nnf.sizeof],
+  rw [add_assoc],
+  rw [nat.one_add],
+  apply nat.lt_succ_self 
+end
+
+theorem split_lt_and_seqt {φ ψ} (Γ : sseqt) (h : nnf.and φ ψ ∈ Γ.m) :
+prod.measure_lex' sseqt_size 
+(and_child Γ h) Γ :=
+begin
+right, right,
+simp only [and_child],
+apply split_lt_and_size _ h
+end
+
+theorem split_lt_or_size_left {φ ψ} (Γ : list nnf) (h : nnf.or φ ψ ∈ Γ) :
+node_size (φ :: Γ.erase (nnf.or φ ψ)) < node_size Γ := 
+begin
+  dsimp,
+  rw ←size_erase_add_eq_size_sum Γ,
+  swap, exact h,
+  rw [add_comm],
+  apply add_lt_add_left, dsimp [sizeof, has_sizeof.sizeof, nnf.sizeof],
+  rw [add_comm, ←add_assoc],
+  apply nat.lt_add_of_pos_left,
+  apply nat.succ_pos
+end
+
+theorem split_lt_or_size_right {φ ψ} (Γ : list nnf) (h : nnf.or φ ψ ∈ Γ) :
+node_size (ψ :: Γ.erase (nnf.or φ ψ)) < node_size Γ := 
+begin
+  dsimp,
+  rw ←size_erase_add_eq_size_sum Γ,
+  swap, exact h,
+  rw [add_comm],
+  apply add_lt_add_left, dsimp [sizeof, has_sizeof.sizeof, nnf.sizeof],
+  apply nat.lt_add_of_pos_left,
+  rw nat.one_add,
+  apply nat.succ_pos
+end
+
+-- theorem split_lt_or_seqt_left {φ ψ} (Γ : seqt) (h : nnf.or φ ψ ∈ Γ.main) :
+-- prod.measure_lex seqt_size (or_child_left Γ h) Γ :=
+-- begin
+--   have hmem : or φ ψ ∈ Γ.main ++ Γ.hdld, {apply mem_append_left _ h},
+--   have := lt_or_eq_of_le (split_le_or_degree_left _ hmem),
+--   cases this,
+--   {left, simp only [seqt_size, or_child_left],  rw erase_append_left at this, rw cons_append, exact this, exact h},
+--   {dsimp only [prod.measure_lex, inv_image, seqt_size], rw [erase_append_left _ h] at this, rw ←this, right,
+--    apply split_lt_or_size_left _ h}
+-- end
+
+-- theorem split_lt_or_seqt_right {φ ψ} (Γ : seqt) (h : nnf.or φ ψ ∈ Γ.main) :
+-- prod.measure_lex seqt_size (or_child_right Γ h) Γ :=
+-- begin
+--   have hmem : or φ ψ ∈ Γ.main ++ Γ.hdld, {apply mem_append_left _ h},
+--   have := lt_or_eq_of_le (split_le_or_degree_right _ hmem),
+--   cases this,
+--   {left, simp only [seqt_size, or_child_right],  rw erase_append_left at this, rw cons_append, exact this, exact h},
+--   {dsimp only [prod.measure_lex, inv_image, seqt_size], rw [erase_append_left _ h] at this, rw ←this, right,
+--    apply split_lt_or_size_right _ h}
+-- end
+
+theorem copy_lt_size {φ} (Γ : list nnf) (h : nnf.box φ ∈ Γ) :
+node_size (φ :: Γ.erase (nnf.box φ)) < node_size Γ := 
+begin
+  dsimp [node_size],
+  rw ←size_erase_add_eq_size_sum Γ,
+  swap, exact h, 
+  rw [add_comm], simp [sizeof,has_sizeof.sizeof, nnf.sizeof], 
+  apply nat.lt_succ_self 
+end
+
+theorem copy_lt_seqt {φ} (Γ : sseqt) (h : nnf.box φ ∈ Γ.m) :
+prod.measure_lex' sseqt_size (box_child Γ h) Γ := 
+begin
+right, right,
+simp only [box_child],
+apply copy_lt_size _ h
+end
+
+theorem box_new_lt_seqt {φ} (Γ : sseqt) 
+(h₁ : nnf.box φ ∈ Γ.m) (h₂ : nnf.box φ ∉ Γ.b) :
+prod.measure_lex' sseqt_size (box_child_new Γ h₁ h₂) Γ := 
+begin
+left,
+apply length_sub_lt_of_nodup_subperm,
+{dsimp [box_child_new], exact Γ.spb},
+{dsimp [box_child_new], apply Γ.sbm, exact h₁},
+{exact h₂},
+{exact Γ.ndb}
+end
